theories/hoare.v
@@ -46,42 +46,67 @@ Admitted.
 
 Lemma get_new_vertex'_fact {T: Type} :
   forall P,
-  Hoare P (@get_new_vertex' T) (
-                                fun n s =>
-                                  exists s',
-                                  n = s.(max_v') /\
-                                  s.(max_v') = s'.(max_v') + 1 /\
-                                  s.(max_e') = s'.(max_e') /\
-                                  s.(st_graph) = s'.(st_graph) /\
-                                  P s'
-                               ).
+  Hoare P
+        (@get_new_vertex' T)
+        (fun n s =>
+          n = s.(max_v') /\
+          exists s',
+          s.(max_v') = s'.(max_v') + 1 /\
+          s.(max_e') = s'.(max_e') /\
+          s.(st_graph) = s'.(st_graph) /\
+          P s'
+        ).
 Proof.
 unfold get_new_vertex', Hoare.
 split; intros.
-- eexists σ1.
-  destruct H0 as [?[?[?]]].
-  repeat split; auto.
+- destruct H0 as [?[?[?]]].
+  split; eauto.
 - eauto.
+Qed.
+
+Lemma pregraph_add_vertex'_fact {T: Type} :
+  forall v P,
+  Hoare (fun s => v = s.(max_v') /\ P s)
+        (@pregraph_add_vertex' T v)
+        (fun G s =>
+          exists s',
+          G = s.(st_graph) /\
+          s.(max_v') = s'.(max_v') /\
+          s.(max_e') = s'.(max_e') /\
+          G_add_vertex s'.(st_graph) v s.(st_graph) /\
+          P s'
+        ).
+Proof.
+unfold pregraph_add_vertex', Hoare.
+split; intros.
+- eexists σ1.
+  destruct H.
+  destruct H0 as [?[?[?]]].
+  destruct H3 as [?[?[?[?[?]]]]].
+  repeat split; eauto.
+  apply H5. apply H5.
+  apply H6. apply H6.
+- destruct H.
+  destruct H0. eauto.
 Qed.
 
 Lemma pregraph_add_whole_vertex'_fact {T: Type} :
   forall P,
   Hoare P
         (v <- @get_new_vertex' T ;; pregraph_add_vertex' v)
-        (
-          fun G s =>
-            exists s',
-            G = s.(st_graph) /\
-            s.(max_v') = s'.(max_v') + 1 /\
-            s.(max_e') = s'.(max_e') /\
-            G_add_vertex s'.(st_graph) s.(max_v') s.(st_graph) /\
-            P s'
+        (fun G s =>
+          exists s',
+          G = s.(st_graph) /\
+          s.(max_v') = s'.(max_v') + 1 /\
+          s.(max_e') = s'.(max_e') /\
+          G_add_vertex s'.(st_graph) s.(max_v') s.(st_graph) /\
+          P s'
         ).
 Proof.
 intros. eapply Hoare_bind. 1 : { apply get_new_vertex'_fact. }
 intros. unfold pregraph_add_vertex', Hoare.
 split; intros.
-- destruct H as [?[?[?[?[]]]]].
+- destruct H as [?[?[?[?[?]]]]].
   destruct H0 as [?[?[?]]].
   eexists x.
   split. eauto.
@@ -100,7 +125,9 @@ Lemma st_graph_refine {T: Type} :
   Hoare (
           fun s1 =>
             (** safeExec_X P_abs c_abs X *)
-            (safeExec (fun s => s.(max_v) = s1.(max_v') /\ s.(max_e) = s1.(max_e'))
+            (safeExec (fun s =>
+                        s.(max_v) = s1.(max_v') /\
+                        s.(max_e) = s1.(max_e'))
                       (regexToNFA r)
                       X) /\
             (*** P_con *)
@@ -112,13 +139,14 @@ Lemma st_graph_refine {T: Type} :
         ( 
           fun '(sv, ev) s2 =>
             (** ∃ a, safeExec_X Q_abs(a) skip *)
-            exists el, (safeExec (
-                                   fun s => s.(max_v) = s2.(max_v') /\
-                                            s.(max_e) = s2.(max_e')
-                                 )
-                                 (return el) (*? skip *)
-                                 X
-                       ) /\
+            exists el,
+            (safeExec (fun s =>
+                        s.(max_v) = s2.(max_v') /\
+                        s.(max_e) = s2.(max_e')
+                      )
+                      (return el) (*? skip *)
+                      X
+            ) /\
             (*? *)
             (forall n, el.(graph).(pg).(vvalid) n -> n <= s2.(max_v')) /\
             (forall n, el.(graph).(pg).(evalid) n -> n <= s2.(max_e')) /\
@@ -129,11 +157,26 @@ Lemma st_graph_refine {T: Type} :
         ).
 Proof.
 induction r.
-- intros. simpl regexToNFA'.
-  intros. eapply Hoare_bind. 1 : { apply get_new_vertex'_fact. }
-  intros. eapply Hoare_bind.
+- simpl regexToNFA'.
+  intros. eapply Hoare_bind. 1 : { eapply get_new_vertex'_fact. }
+  intros. eapply Hoare_bind. 1 : { eapply pregraph_add_vertex'_fact. }
+  intros. eapply Hoare_bind. 1 : { eapply get_new_vertex'_fact. }
+  intros. eapply Hoare_bind. 1 : { eapply pregraph_add_vertex'_fact. }
+  intros. eapply Hoare_return. 1 : {
+    intros.
+    destruct H as [?[?[?[?]]]].
+    destruct H2 as [?[?[?[?[?]]]]].
+    (** eexists (Build_elem a a1 ... ) *)
+    eexists (@Build_elem T a a1 (emptyset_nfa a a1)).
+    simpl. repeat split; eauto.
+    - destruct H6 as [?[?[?[?[?[?[?[?[?[?[? [? ?]]]]]]]]]]]].
+      unfold emptyset_nfa. unfold regexToNFA, act_empty in H13.
+      eapply highstepbind_derive in H13.
+      2 : { instantiate (1 := x1.(max_v')). }
+      (** x2 -<new_v'>- x1 -<+a>- x0 -<new_v'>- x -<+a1>- σ *)
+
 Admitted.
 
+Check Build_elem.
+
 Check safeExec.
-
-
